Remove almost all axioms (#163)
Depends on https://github.com/dafny-lang/Dafny-VMC/pull/161 and
https://github.com/dafny-lang/Dafny-VMC/pull/162

By submitting this pull request, I confirm that my contribution is made
under the terms of the [MIT
license](https://github.com/dafny-lang/dafny/blob/master/LICENSE.txt).

src/Distributions/Uniform/Correctness.dfy
@@ -16,6 +16,17 @@ module Uniform.Correctness {
    Definitions
   ************/
 
+  function IntervalSampleIsIndepFunctionHelper(a: int, x: int): nat
+    requires x-a >= 0
+  {
+    x-a
+  }
+
+  ghost function IntervalSampleIsIndepFunctionHelperLifted(a: int, A: iset<int>): iset<nat>
+  {
+    iset x: int | x in A && x-a >= 0 :: IntervalSampleIsIndepFunctionHelper(a, x)
+  }
+
   ghost function SampleEquals(n: nat, i: nat): iset<Rand.Bitstream>
     requires 0 <= i < n
   {
@@ -28,10 +39,13 @@ module Uniform.Correctness {
 
   // Correctness theorem for Model.Sample
   // Equation (4.12) / PROB_BERN_UNIFORM
-  lemma {:axiom} UniformFullCorrectness(n: nat, i: nat)
+  lemma UniformFullCorrectness(n: nat, i: nat)
     requires 0 <= i < n
-    ensures SampleEquals(n, i) in Rand.eventSpace
-    ensures Rand.prob(SampleEquals(n, i)) == 1.0 / (n as real)
+    ensures
+      var e := iset s | Model.Sample(n)(s).Equals(i);
+      e in Rand.eventSpace &&
+      Rand.prob(e) == 1.0 / (n as real)
+  {}
 
   // Correctness theorem for Model.IntervalSample
   lemma UniformFullIntervalCorrectness(a: int, b: int, i: int)
@@ -55,17 +69,96 @@ module Uniform.Correctness {
     }
   }
 
-  // Equation (4.10)
-  lemma SampleIsIndep(n: nat)
+  lemma SampleIsIndepFunction(n: nat)
     requires n > 0
-    ensures Independence.IsIndep(Model.Sample(n))
+    ensures Independence.IsIndepFunction(Model.Sample(n))
   {}
 
-  lemma IntervalSampleIsIndep(a: int, b: int)
+  lemma IntervalSampleIsIndepFunction(a: int, b: int)
     requires a < b
-    ensures Independence.IsIndep(Model.IntervalSample(a, b))
+    ensures Independence.IsIndepFunction(Model.IntervalSample(a, b))
   {
-    SampleIsIndep(b-a);
-    Independence.MapIsIndep(Model.Sample(b-a), x => a + x);
+    forall A: iset<int>, E: iset<Rand.Bitstream> | E in Rand.eventSpace ensures Independence.IsIndepFunctionCondition(Model.IntervalSample(a, b), A, E) {
+      var A': iset<nat> := IntervalSampleIsIndepFunctionHelperLifted(a, A);
+      assert Measures.AreIndepEvents(Rand.eventSpace, Rand.prob, Monad.BitstreamsWithValueIn(Model.IntervalSample(a, b), A), Monad.BitstreamsWithRestIn(Model.IntervalSample(a, b), E)) by {
+        assert Monad.BitstreamsWithValueIn(Model.IntervalSample(a, b), A) == Monad.BitstreamsWithValueIn(Model.Sample(b - a), A') by {
+          forall s ensures s in Monad.BitstreamsWithValueIn(Model.IntervalSample(a, b), A) <==> s in Monad.BitstreamsWithValueIn(Model.Sample(b - a), A') {
+            calc {
+              s in Monad.BitstreamsWithValueIn(Model.IntervalSample(a, b), A);
+              Monad.Map(Model.Sample(b - a), x => a + x)(s).value in A;
+              Monad.Bind(Model.Sample(b - a), x => Monad.Return(a+x))(s).value in A;
+              Model.Sample(b - a)(s).value + a in A;
+              Model.Sample(b - a)(s).value in A';
+              s in Monad.BitstreamsWithValueIn(Model.Sample(b - a), A');
+            }
+          }
+        }
+        assert Monad.BitstreamsWithRestIn(Model.IntervalSample(a, b), E) == Monad.BitstreamsWithRestIn(Model.Sample(b-a), E) by {
+          forall s ensures s in Monad.BitstreamsWithRestIn(Model.IntervalSample(a, b), E) <==> s in Monad.BitstreamsWithRestIn(Model.Sample(b-a), E) {
+            calc {
+              s in Monad.BitstreamsWithRestIn(Model.IntervalSample(a, b), E);
+              Monad.Map(Model.Sample(b - a), x => a + x)(s).rest in E;
+              Monad.Bind(Model.Sample(b - a), x => Monad.Return(a+x))(s).rest in E;
+              Model.Sample(b-a)(s).rest in E;
+              s in Monad.BitstreamsWithRestIn(Model.Sample(b-a), E);
+            }
+          }
+        }
+        assert Independence.IsIndepFunctionCondition(Model.Sample(b - a), A', E) by {
+          SampleIsIndepFunction(b-a);
+        }
+      }
+    }
+  }
+
+  lemma SampleBound(n: nat, s: Rand.Bitstream)
+    requires n > 0
+    ensures 0 <= Model.Sample(n)(s).value < n
+  {}
+
+  lemma IntervalSampleBound(a: int, b: int, s: Rand.Bitstream)
+    requires a < b
+    ensures a <= Model.IntervalSample(a, b)(s).value < b
+  {
+    SampleBound(b-a, s);
+  }
+
+  lemma SampleIsMeasurePreserving(n: nat)
+    requires n > 0
+    ensures forall n | n > 0 :: Measures.IsMeasurePreserving(Rand.eventSpace, Rand.prob, Rand.eventSpace, Rand.prob, s => Model.Sample(n)(s).rest)
+  {}
+
+  lemma IntervalSampleIsMeasurePreserving(a: int, b: int)
+    requires a < b
+    ensures Measures.IsMeasurePreserving(Rand.eventSpace, Rand.prob, Rand.eventSpace, Rand.prob, s => Model.IntervalSample(a, b)(s).rest)
+  {
+    var f := s => Model.IntervalSample(a, b)(s).rest;
+    var f' := s => Model.Sample(b-a)(s).rest;
+
+    forall e: iset<Rand.Bitstream> | e in Rand.eventSpace ensures Measures.PreImage(f, e) == Measures.PreImage(f', e) {
+      forall s ensures s in Measures.PreImage(f, e) <==> s in Measures.PreImage(f', e) {
+        calc {
+          s in Measures.PreImage(f, e);
+          f(s) in e;
+          Model.IntervalSample(a, b)(s).rest in e;
+          Model.Sample(b-a)(s).rest in e;
+          f'(s) in e;
+          s in Measures.PreImage(f', e);
+        }
+      }
+    }
+
+    assert Measures.IsMeasurable(Rand.eventSpace, Rand.eventSpace, f) by {
+      forall e: iset<Rand.Bitstream> | e in Rand.eventSpace ensures Measures.PreImage(f, e) in Rand.eventSpace {
+        assert Measures.PreImage(f, e) == Measures.PreImage(f', e);
+        SampleIsMeasurePreserving(b-a);
+      }
+    }
+
+    forall e | e in Rand.eventSpace ensures Rand.prob(Measures.PreImage(f, e)) == Rand.prob(e) {
+      assert Measures.PreImage(f, e) == Measures.PreImage(f', e);
+      SampleIsMeasurePreserving(b-a);
+    }
+
   }
 }
