src/Distributions/Uniform/Model.dfy
@@ -16,35 +16,20 @@ module Uniform.Model {
   ************/
 
   // Definition 49
-  opaque ghost function {:axiom} Sample(n: nat): (h: Monad.Hurd<nat>)
+  ghost function {:axiom} Sample(n: nat): (h: Monad.Hurd<nat>)
     requires n > 0
-    ensures Independence.IsIndep(h)
+    ensures Independence.IsIndepFunction(h)
+    ensures Measures.IsMeasurePreserving(Rand.eventSpace, Rand.prob, Rand.eventSpace, Rand.prob, s => h(s).rest)
     ensures forall s :: 0 <= h(s).value < n
+    ensures forall i | 0 <= i < n ::
+              var e := iset s | h(s).Equals(i);
+              && e in Rand.eventSpace
+              && Rand.prob(e) == 1.0 / (n as real)
 
   ghost function IntervalSample(a: int, b: int): (f: Monad.Hurd<int>)
     requires a < b
   {
     Monad.Map(Sample(b - a), x => a + x)
   }
-
-  /*******
-   Lemmas
-  *******/
-
-  lemma SampleBound(n: nat, s: Rand.Bitstream)
-    requires n > 0
-    ensures 0 <= Sample(n)(s).value < n
-  {}
-
-  lemma IntervalSampleBound(a: int, b: int, s: Rand.Bitstream)
-    requires a < b
-    ensures a <= IntervalSample(a, b)(s).value < b
-  {
-    SampleBound(b-a, s);
-  }
-
-  lemma {:axiom} IntervalSampleIsMeasurePreserving(a: int, b: int)
-    requires a < b
-    ensures Measures.IsMeasurePreserving(Rand.eventSpace, Rand.prob, Rand.eventSpace, Rand.prob, s => IntervalSample(a, b)(s).rest)
 
 }
